src/Distributions/UniformPowerOfTwo/Model.dfy
@@ -36,7 +36,7 @@ module UniformPowerOfTwo.Model {
   {
     (s: Rand.Bitstream) =>
       if n == 1 then
-        (u, s)
+        Monad.Result(u, s)
       else
         SampleTailRecursive(n / 2, if Monad.Head(s) then 2*u + 1 else 2*u)(Monad.Tail(s))
   }
@@ -118,7 +118,7 @@ module UniformPowerOfTwo.Model {
     if l == 0 {
       calc {
         Monad.Bind(Sample(Helper.Power(2, m)), (u: nat) => SampleTailRecursive(Helper.Power(2, l), u))(s);
-        (var (u, s') := Sample(Helper.Power(2, m))(s); SampleTailRecursive(1, u)(s'));
+        (var Result(u, s') := Sample(Helper.Power(2, m))(s); SampleTailRecursive(1, u)(s'));
         Sample(Helper.Power(2, m + l))(s);
       }
     } else {
@@ -127,15 +127,15 @@ module UniformPowerOfTwo.Model {
       assert L1GreaterZero: Helper.Power(2, l - 1) >= 1 by { Helper.PowerGreater0(2, l - 1); }
       calc {
         Monad.Bind(Sample(Helper.Power(2, m)), (u: nat) => SampleTailRecursive(Helper.Power(2, l), u))(s);
-        (var (u, s') := Sample(Helper.Power(2, m))(s); SampleTailRecursive(Helper.Power(2, l), u)(s'));
+        (var Result(u, s') := Sample(Helper.Power(2, m))(s); SampleTailRecursive(Helper.Power(2, l), u)(s'));
         { reveal LGreaterZero; }
-        (var (u, s') := Sample(Helper.Power(2, m))(s);
+        (var Result(u, s') := Sample(Helper.Power(2, m))(s);
          SampleTailRecursive(Helper.Power(2, l) / 2, if Monad.Head(s') then 2 * u + 1 else 2 * u)(Monad.Tail(s')));
         { assert Helper.Power(2, l) / 2 == Helper.Power(2, l - 1); reveal L1GreaterZero; }
-        (var (u', s') := Monad.Bind(Sample(Helper.Power(2, m)), UnifStep)(s);
+        (var Result(u', s') := Monad.Bind(Sample(Helper.Power(2, m)), UnifStep)(s);
          SampleTailRecursive(Helper.Power(2, l - 1), u')(s'));
         { assert Helper.Power(2, m + 1) / 2 == Helper.Power(2, m); }
-        (var (u', s') := Sample(Helper.Power(2, m + 1))(s);
+        (var Result(u', s') := Sample(Helper.Power(2, m + 1))(s);
          SampleTailRecursive(Helper.Power(2, l - 1), u')(s'));
         Monad.Bind(Sample(Helper.Power(2, m + 1)), (u: nat) => SampleTailRecursive(Helper.Power(2, l - 1), u))(s);
         { RelateWithTailRecursive(l - 1, m + 1, s); }
