src/ProbabilisticProgramming/Loops.dfy
@@ -46,7 +46,7 @@ module Loops {
         WhileCut(condition, body, init, fuel)(s)
       else
         // In HOL, Hurd returns `arb` here, which is not possible in Dafny.
-        (init, s)
+        Monad.Result(init, s)
   }
 
   ghost function LeastFuel<A>(condition: A -> bool, body: A -> Monad.Hurd<A>, init: A, s: Rand.Bitstream): (fuel: nat)
@@ -132,7 +132,7 @@ module Loops {
     requires WhileCutTerminates(condition, body, init', s')
     requires LeastFuel(condition, body, init', s') == fuel'
     requires condition(init)
-    requires body(init)(s) == (init', s')
+    requires body(init)(s) == Monad.Result(init', s')
     ensures WhileCutTerminates(condition, body, init, s)
     ensures LeastFuel(condition, body, init, s) == fuel' + 1
   {
@@ -148,21 +148,21 @@ module Loops {
 
   lemma WhileCutUnroll<A>(condition: A -> bool, body: A -> Monad.Hurd<A>, init: A, s: Rand.Bitstream, init': A, s': Rand.Bitstream, fuel: nat)
     requires condition(init)
-    requires body(init)(s) == (init', s')
+    requires body(init)(s) == Monad.Result(init', s')
     ensures WhileCut(condition, body, init, fuel + 1)(s) == WhileCut(condition, body, init', fuel)(s')
   {}
 
 
   lemma WhileCutTerminatesWithFuelUnroll<A>(condition: A -> bool, body: A -> Monad.Hurd<A>, init: A, s: Rand.Bitstream, init': A, s': Rand.Bitstream, fuel: nat)
     requires condition(init)
-    requires body(init)(s) == (init', s')
+    requires body(init)(s) == Monad.Result(init', s')
     ensures WhileCutTerminatesWithFuel(condition, body, init, s)(fuel + 1) == WhileCutTerminatesWithFuel(condition, body, init', s')(fuel)
   {}
 
-  lemma WhileUnrollIfConditionSatisfied<A>(condition: A -> bool, body: A -> Monad.Hurd<A>, init: A, s: Rand.Bitstream, init': A, s': Rand.Bitstream, loop: (A, Rand.Bitstream), unrolled: (A, Rand.Bitstream))
+  lemma WhileUnrollIfConditionSatisfied<A>(condition: A -> bool, body: A -> Monad.Hurd<A>, init: A, s: Rand.Bitstream, init': A, s': Rand.Bitstream, loop: Monad.Result<A>, unrolled: Monad.Result<A>)
     requires WhileCutTerminates(condition, body, init, s)
     requires condition(init)
-    requires body(init)(s) == (init', s')
+    requires body(init)(s) == Monad.Result(init', s')
     requires loop == While(condition, body, init)(s)
     requires unrolled == While(condition, body, init')(s')
     ensures loop == unrolled
@@ -187,7 +187,7 @@ module Loops {
     }
   }
 
-  lemma WhileUnrollIfTerminates<A>(condition: A -> bool, body: A -> Monad.Hurd<A>, init: A, s: Rand.Bitstream, fuel: nat, loop: (A, Rand.Bitstream), unrolled: (A, Rand.Bitstream))
+  lemma WhileUnrollIfTerminates<A>(condition: A -> bool, body: A -> Monad.Hurd<A>, init: A, s: Rand.Bitstream, fuel: nat, loop: Monad.Result<A>, unrolled: Monad.Result<A>)
     requires WhileCutTerminates(condition, body, init, s)
     requires fuel == LeastFuel(condition, body, init, s)
     requires loop == While(condition, body, init)(s)
@@ -195,7 +195,7 @@ module Loops {
     ensures loop == unrolled
   {
     if condition(init) {
-      var (init', s') := body(init)(s);
+      var Result(init', s') := body(init)(s);
       calc {
         loop;
         { WhileUnrollIfConditionSatisfied(condition, body, init, s, init', s', loop, unrolled); }
@@ -205,7 +205,7 @@ module Loops {
     } else {
       calc {
         loop;
-        (init, s);
+        Monad.Result(init, s);
         unrolled;
       }
     }
@@ -279,7 +279,7 @@ module Loops {
   {
     var reject := (a: A) => !accept(a);
     var body := (a: A) => proposal;
-    var (init, s') := proposal(s);
+    var Result(init, s') := proposal(s);
     WhileUnroll(reject, body, init, s');
   }
 
